\documentclass{article}
\usepackage{amsmath}
\usepackage{amsthm}
\usepackage{amssymb}
\usepackage[a4paper, left=1.5cm, right=1.5cm, top=2.5cm, bottom=2.5cm]{geometry}
\usepackage{tikz}
\usetikzlibrary{tikzmark}
\usepackage{stata}

\title{PS1}

\begin{document}
\maketitle
\begin{enumerate}
    \item \begin{enumerate}
        \item \begin{proof}
            \begin{equation}
                \begin{aligned}
                    \sum_{i=1}^{n}y_i
                    &=\sum_{i=1}^{n}(x_{i1}+1-x_{i1})\times y_i \\
                    &=\sum_{i=1}^{n}x_{i1}\times y_i+\sum_{i=1}^{n}(1-x_{i1})\times y_i \\
                \end{aligned}
                \nonumber
            \end{equation}
        \end{proof}
        \item \begin{equation}
            \begin{aligned}
                \hat{\beta}_1
                &=\frac{\sum_{i=1}^{n}(x_{i1}-\overline{x})(y_i-\overline{y})}{\sum_{i=1}^{n}(x_{i1}-\overline{x})^2} \\
                &=\frac{\sum_{i=1}^{n}x_{i1}y_i-\overline{x}\sum_{i=1}^{n}y_i-\overline{y}\sum_{i=1}^{n}x_{1i}+\sum_{i=1}^{n}\overline{x}\overline{y}}{\sum_{i=1}^{n}x_{1i}-2\overline{x}\sum_{i=1}^{n}x_{1i}+\overline{x}\sum_{i=1}^{n}x_{1i}} \\
                &=\frac{\sum_{i=1}^{n}x_{i1}y_i-\overline{x}\sum_{i=1}^{n}y_i-\overline{y}\sum_{i=1}^{n}x_{1i}+\overline{x}\sum_{i=1}^{n}y_i}{(1-\overline{x})\sum_{i=1}^{n}x_{1i}} \\
                &=\frac{\sum_{i=1}^{n}x_{i1}y_i-\overline{y}\sum_{i=1}^{n}x_{1i}}{(1-\overline{x})\sum_{i=1}^{n}x_{1i}} \\
                &=\frac{\sum_{i=1}^{n}x_{i1}y_i}{(1-\overline{x})\sum_{i=1}^{n}x_{1i}}-\frac{\overline{y}}{1-\overline{x}} \\
                &=\frac{\sum_{i=1}^{n}x_{i1}y_i}{(1-\overline{x})\sum_{i=1}^{n}x_{1i}}-\frac{\sum_{i=1}^{n}y_i}{\sum_{i=1}^{n}(1-x_{i1})} \\
                &=\frac{\sum_{i=1}^{n}x_{i1}y_i}{(1-\overline{x})\sum_{i=1}^{n}x_{1i}}-\frac{\sum_{i=1}^{n}x_{i1}y_i}{\sum_{i=1}^{n}(1-x_{i1})}-\frac{\sum_{i=1}^{n}(1-x_{i1})y_i}{\sum_{i=1}^{n}(1-x_{i1})} \\
                &=\left(\sum_{i=1}^{n}x_{i1}y_i\right)\left(\frac{1}{(1-\overline{x})\sum_{i=1}^{n}x_{1i}}-\frac{1}{\sum_{i=1}^{n}(1-x_{i1})}\right)-\frac{\sum_{i=1}^{n}(1-x_{i1})y_i}{n_0} \\
                &=\left(\sum_{i=1}^{n}x_{i1}y_i\right)\frac{n-\sum_{i=1}^{n}x_{1i}}{\sum_{i=1}^{n}(1-x_{1i})\sum_{i=1}^{n}x_{1i}}-\overline{y}_0 \\
                &=\frac{\sum_{i=1}^{n}x_{i1}y_i}{\sum_{i=1}^{n}x_{1i}}-\overline{y}_0 \\
                &=\overline{y}_1-\overline{y}_0 \\
                \hat{\beta}_0
                &=\overline{y}-\hat{\beta}_1\overline{x} \\
                &=\frac{\sum_{i=1}^{n}y_i}{n}-(\overline{y}_1-\overline{y}_0)\frac{\sum_{i=1}^{n}x_{1i}}{n} \\
                &=\overline{y}_0\frac{\sum_{i=1}^{n}x_{1i}}{n}+\frac{\sum_{i=1}^{n}y_i}{n}-\frac{\overline{y}_1\sum_{i=1}^{n}x_{1i}}{n} \\
                &=\overline{y}_0\frac{\sum_{i=1}^{n}x_{1i}}{n}+\frac{\sum_{i=1}^{n}y_i}{n}-\frac{\overline{y}_1\times n_1}{n} \\
                &=\overline{y}_0\frac{\sum_{i=1}^{n}x_{1i}}{n}+\frac{\sum_{i=1}^{n}(1-x_{i1})y_i}{n} \\
                &=\overline{y}_0\frac{\sum_{i=1}^{n}x_{1i}}{n}+\overline{y}_0\frac{\sum_{i=1}^{n}(1-x_{1i})}{n} \\
                &=\overline{y}_0
            \end{aligned}
            \nonumber
        \end{equation}
        \item $\hat{\beta}_1$ represents the difference between y on $x=1$ and y on $x=0$, and $\hat{\beta}_0$ represents the average of y on $x=0$.
        \item \begin{proof}
            \begin{equation}
                \begin{aligned}
                    \mathbb{E}[\hat{\beta}_1]
                    &=\beta_1 \\
                    &=\frac{\mathbb{E}[y]-\beta_0}{\mathbb{E}[x_1]} \\
                    &=\frac{\mathbb{E}[y|x_1=1]P(x_1=1)+\mathbb{E}[y|x_1=0]P(x_1=0)-\mathbb{E}[y|x_1=0]}{P(x_1=0)\times0+P(x_1=1)\times1} \\
                    &=\frac{\mathbb{E}[y|x_1=1]P(x_1=1)-\mathbb{E}[y|x_1=0]P(x_1=1)}{P(x_1=1)} \\
                    &=\mathbb{E}[y|x_1=1]-\mathbb{E}[y|x_1=0] \\
                \end{aligned}
                \nonumber
            \end{equation}
        \end{proof}
    \end{enumerate}
    \item \begin{enumerate}
        \item There's 3 possible explanations for the correlation between smoking and baby's weight.
        \begin{enumerate}
            \item The more the mother smoked, the less the baby's weight.
            \item The less the baby's weight, the more the mother smoked.
            \item There's a third variable that affects both the mother's smoking and the baby's weight in the contrary way.
        \end{enumerate}
        \item Because the more the mother smoked, the less the baby's weight, and the effect of smoking on baby's weight is quite big.
        \item Yes, it's possible according to the common sense.
    \end{enumerate}
    \item \begin{enumerate}
        \item \begin{stlog}
            \input{Q3a.log}
        \end{stlog}
        \item \begin{stlog}
            \input{Q3b.log}
        \end{stlog} \par
        Female in the sample accounts for 29.85\%.
        \item \begin{stlog}
            \input{Q3c.log}
        \end{stlog} \par
        So, we have $\text{wage}=62580.26-14935.5\times\text{female}$ . \par
        Using my conclusion in Q1, this regression result means that 
        the wage difference between female and male is $-14935.5$ yuan, 
        and the average wage for male is $62580.26$ yuan.
        \item \begin{stlog}
            \input{Q3d.log}
        \end{stlog} \par
        If \textbf{\texttt{schooling\_yr}} increases by 1, the \textbf{log(\texttt{wage})} will increase by 0.043.
        \item \begin{stlog}
            \input{Q3e.log}
        \end{stlog} \par
        The residual is very small, which suggests that the model fits the data well.
        \item In (d) , we have $R^2=0.0265$ , indicating that there may be other factors not included in the model.
    \end{enumerate}
\end{enumerate}
\end{document}